\documentclass[11pt]{article}
\usepackage[utf8]{inputenc}
\usepackage{amsfonts}
\usepackage{amsmath}
\usepackage{float}

\setlength{\parindent}{0em}
\setlength{\parskip}{1em}

\usepackage{geometry}
\geometry{
  a4paper,
  total={170mm,257mm},
  left=20mm,
  top=20mm,
}

\makeatletter
\newcommand{\mathleft}{\@fleqntrue\@mathmargin5pt}
\newcommand{\mathcenter}{\@fleqnfalse}
\makeatother

\title{Labsheet 1.3}
\author{Rowan Saunders}
\begin{document}

\maketitle

\section{Exercise 1}
\begin{itemize}
  \item[a)] $x$ is a variable
  \item[b)] $\lambda x.x$ is an abstraction
  \item[c)] $(\lambda a.z)a$ is an application
  \item[d)] $\lambda a.za$ is an abstraction
  \item[e)] $(\lambda n.n)z$ is an application
  \item[f)] $\lambda z.(\lambda y.(\lambda x.x)y)z$ is an abstraction
  \item[g)] $(\lambda t.((\lambda t.(\lambda t.t)t)t))t$ is an application
\end{itemize}

\section{Exercise 2}
\begin{itemize}
  \item[a)] $(\lambda x.xy)[\lambda z.z / y] == (\lambda x.x(\lambda z.z))$
  \item[b)] $(\lambda x.xy)[\lambda z.zx / y] \to_\alpha (\lambda w.wy)[\lambda
    z.zx / y] == \lambda w.w(\lambda z.zx)$
  \item[c)] $(f(\lambda x.yx)yx)[fy / x] \to_\alpha (f (\lambda z.yz)yx)[fy / x]
    == (f(\lambda z.yz)y(fy))$
  \item[d)] $(\lambda f.f(\lambda x.yx)yx)[fy / x] \to_\alpha (\lambda
    z.z(\lambda w.yw)yx)[fy / x] == (\lambda z.z(\lambda w.yw)y(fy))$
\end{itemize}

\section{Exercise 3}
\begin{itemize}
  \item[a)] $(\lambda x.\lambda y.x) yx \to_\beta (\lambda z.y)x$
  \item[b)] $(\lambda f.f(\lambda x.x))(\lambda y.z) \to_\beta (\lambda
    y.z)(\lambda x.x)$
  \item[c)] $(\lambda x.\lambda y.yx)(\lambda x.xy) \to_\alpha (\lambda
    w.\lambda z.zw)(\lambda x.xy) \to_\beta \lambda z.z(\lambda x.xy)$
  \item[d)] $(\lambda x.xx)((\lambda y.y)(\lambda x.x)) \to_\beta (\lambda
    x.xx)(\lambda x.x) \to_\beta (\lambda x.x)(\lambda x.x) \to_\beta \lambda
    x.x$
  \item[e)] $(\lambda x.xx)(\lambda y.y)(\lambda x.x) \to_\beta (\lambda
    y.y)(\lambda y.y)(\lambda x.x) \to_\beta (\lambda y.y)(\lambda x.x)
    \to_\beta (\lambda x.x)$
  \item[f)] $(\lambda x.xx)(\lambda x.xx)((\lambda y.y)(\lambda x.x)) \to_\beta
    (\lambda x.xx)(\lambda x.xx)(\lambda x.x) \to_\beta (\lambda x.xx)(\lambda
    x.xx)(\lambda x.x) \to_\beta$
    $(\lambda x.xx)(\lambda x.xx)(\lambda x.x)
    \to_\beta ...$
\end{itemize}

\section{Exercise 4}
\subsection{a)}
$$ M = (\lambda x.\lambda y.xy)z) \to_\beta (\lambda y.zy)$$
$$ N = (\lambda x.x)(\lambda y.zy) \to_\beta (\lambda y.zy)$$
$$ P = (\lambda y.zy)$$

\subsection{b)}



\end{document}
