\documentclass[11pt]{article}
\usepackage[utf8]{inputenc}
\usepackage{amsfonts}
\usepackage{amsmath}
\usepackage{float}

\setlength{\parindent}{0em}
\setlength{\parskip}{1em}

\usepackage{geometry}
\geometry{
  a4paper,
  total={170mm,257mm},
  left=20mm,
  top=20mm,
}

\makeatletter
\newcommand{\mathleft}{\@fleqntrue\@mathmargin5pt}
\newcommand{\mathcenter}{\@fleqnfalse}
\makeatother

\title{Labsheet 1.3}
\author{Rowan Saunders}
\begin{document}

\maketitle

\section{Exercise 1}

\begin{align*}
  S &= \lambda xyz.xz(yz)\\
  K &= \lambda xy.x\\
  I &= \lambda x.x\\
\end{align*}

\subsection{a)}

\begin{align*}
  SKK &= (\lambda xyz.xz(yz))(\lambda xy.x)(\lambda xy.x)\\
  &\to_\alpha (\lambda xwz.xz(wz))(\lambda xy.x)(\lambda xy.x)\\
  &\to_\beta (\lambda wz.(\lambda xy.x)z(wz))(\lambda xy.x)\\
  &\to_\beta (\lambda z.(\lambda xy.x)z((\lambda xy.x)z))\\
  &\to_\beta (\lambda z.(\lambda xy.x)z(\lambda y.z))\\
  &\to_\beta (\lambda z.(\lambda y.z)(\lambda y.z))\\
  &\to_\beta (\lambda z.z)\\
\end{align*}

\subsection{b)}

\begin{align*}
  SIK =& (\lambda xyz.xz(yz))IK\\
  \to_\beta& (\lambda yz.Iz(yz))K\\
  \to_\beta& (\lambda z.Iz(Kz))\\
  =& (\lambda z.Iz((\lambda xy.x)z))\\
  \to_\beta& (\lambda z.Iz(\lambda y.z))\\
  =& (\lambda z.(\lambda x.x)z(\lambda y.z))\\
  \to_\beta& (\lambda z.z(\lambda y.z))\\
\end{align*}

\subsection{c)}

\begin{align*}
  SSS =& (\lambda xyz.xz(yz))SS\\
  \to_\beta& (\lambda yz.Sz(yz))S\\
  \to_\beta& (\lambda z.Sz(Sz))\\
  =& (\lambda z.(\lambda xyw.xw(yw))z(Sz))\\
  \to_\beta& (\lambda z.(\lambda yw.zw(yw))(Sz))\\
  \to_\beta& (\lambda z.(\lambda w.zw((Sz)w)))\\
  =& (\lambda z.(\lambda w.zw(((\lambda xyk.xk(yk))z)w)))\\
  \to_\beta& (\lambda z.(\lambda w.zw((\lambda yk.zk(yk))w)))\\
  \to_\beta& (\lambda z.(\lambda w.zw(\lambda k.zk(wk))))\\
  =& (\lambda zw.zw(\lambda k.zk(wk)))\\
\end{align*}

\section{Exercise 2}

Let $W$ be the term:
$$ \lambda x.\lambda y.xyy $$

\subsection{a)}
\begin{align*}
  WW =& (\lambda xy.xyy)(\lambda xy.xyy)\\
  \to_\alpha& (\lambda zw.zww)(\lambda xy.xyy)\\
  \to_\beta& (\lambda w.(\lambda xy.xyy)ww)\\
  \to_\beta& (\lambda w.(\lambda y.wyy)w)\\
  \to_\beta& (\lambda w.www)\\
\end{align*}

\subsection{b)}
The term $WWW$ can be reduced to $(\lambda w.www)W$ which with one further beta reduction reduces back to $WWW$
This tells us that $WWW$ does not have a normal form and will only ever reduce to itself.

\end{document}
